pulse/lib/steel/pulse/Pulse.Typing.Metatheory.fsti
@@ -76,3 +76,84 @@ let st_typing_equiv_pre (#g:env) (#t:st_term) (#c:comp_st) (d:st_typing g t c)
                         (veq: vprop_equiv g (comp_pre c) pre)
   : st_typing g t (comp_st_with_pre c pre)
   = admit()
+
+
+///// Substitution lemma /////
+
+module L = FStar.List.Tot
+let map_opt (#a #b:Type) (f:a -> b) (x:option a) : option b =
+  match x with
+  | None -> None
+  | Some x -> Some (f x)
+
+let subst_flip (ss:subst) (t:term) = subst_term t ss
+
+let subst_env (en:env) (ss:subst)
+  : en':env { forall (x:var). lookup en' x ==
+                              map_opt (subst_flip ss) (lookup en x) }
+  = admit ()
+
+type nt_subst = s:subst {
+  forall (elt:subst_elt). List.Tot.memP elt s ==> NT? elt
+}
+
+let pairwise_disjoint (g g' g'':env) =
+  disjoint g g' /\ disjoint g' g'' /\ disjoint g g''
+
+let rec lookup_nt_subst (ss:nt_subst) (x:var) : option term =
+  match ss with
+  | [] -> None
+  | (NT y t)::ss -> if x = y then Some t else lookup_nt_subst ss x
+
+let well_typed_ss (g:env) (g':env) (ss:nt_subst) =
+
+  forall (elt:subst_elt).
+  L.memP elt ss ==> (let NT x e = elt in
+                     x `Set.mem` dom g' /\
+                     (let Some t = lookup g' x in
+                      tot_typing g e t))
+
+let ss_covers_g' (ss:nt_subst) (g':env) =
+  forall (x:var). x `Set.mem` dom g' ==> Some? (lookup_nt_subst ss x)
+
+let tot_typing_subst (g:env) (g':env) (g'':env { pairwise_disjoint g g' g'' })
+  (#e1:term) (#t1:typ)
+  (e1_typing:tot_typing (push_env g (push_env g' g'')) e1 t1)
+  (ss:nt_subst { well_typed_ss g g' ss /\ ss_covers_g' ss g' })
+  : tot_typing (push_env g g'') (subst_term e1 ss) (subst_term t1 ss) = admit ()
+  
+let rec st_typing_subst (g:env) (g':env) (g'':env { pairwise_disjoint g g' g'' })
+  (#e1:st_term) (#c1:comp_st)
+  (e1_typing:st_typing (push_env g (push_env g' g'')) e1 c1)
+  (ss:nt_subst { well_typed_ss g g' ss /\ ss_covers_g' ss g' })
+  : st_typing (push_env g g'') (subst_st_term e1 ss) (subst_comp c1 ss) =
+
+  match e1_typing with
+  | T_Abs _ x q b u body c b_ty_typing body_typing ->
+    let b_ty_typing
+      : tot_typing (push_env g g'')
+                   (subst_term b.binder_ty ss)
+                   (tm_type u) = tot_typing_subst g g' g'' b_ty_typing ss in
+    
+    let g1 : env = push_binding (push_env g (push_env g' g'')) x (subst_term b.binder_ty ss) in
+    let g2 : env = push_env g (push_env g' (push_binding g'' x (subst_term b.binder_ty ss))) in
+    assume (bindings g1 == bindings g2);
+  
+    let body_typing
+      : st_typing g1 (open_st_term_nv (subst_st_term body ss) (b.binder_ppname, x)) (subst_comp c ss)
+      = st_typing_subst g g' (push_binding g'' x (subst_term b.binder_ty ss)) body_typing ss in
+
+    T_Abs (push_env g g') x q (subst_binder b ss) u (subst_st_term body ss) (subst_comp c ss)
+          b_ty_typing body_typing
+
+  | T_STApp _ head ty q res arg head_typing arg_typing ->
+    assume (subst_term (tm_arrow (as_binder ty) q res) ss ==
+            tm_arrow (as_binder (subst_term ty ss)) q (subst_comp res ss));
+    assume (subst_comp (open_comp_with res arg) ss ==
+            open_comp_with (subst_comp res ss) (subst_term arg ss));
+    T_STApp (push_env g g'') (subst_term head ss) (subst_term ty ss) q
+            (subst_comp res ss) (subst_term arg ss)
+            (tot_typing_subst g g' g'' head_typing ss)
+            (tot_typing_subst g g' g'' arg_typing ss)
+
+  | _ -> admit ()
